CoqOfRust/ink/ink.v
@@ -3,8 +3,8 @@ Require Import CoqOfRust.CoqOfRust.
 Require CoqOfRust.ink.ink_env.
 
 Module result_info.
-  Module IsResultType.
-    Section IsResultType.
+  (* Module IsResultType.
+    (* Section IsResultType.
       Context {T : Set}.
       Unset Primitive Projections.
       Record t : Set := {
@@ -18,9 +18,9 @@ Module result_info.
       Global Instance Get_AF_marker : Notation.DoubleColon t "marker" := {
         Notation.double_colon '(Build_t x0) := x0;
       }.
-    End IsResultType.
-  End IsResultType.
-  Definition IsResultType (T : Set) : Set := IsResultType.t (T := T).
+    End IsResultType. *)
+  End IsResultType. *)
+  
   
   Module IsResultTypeFallback.
     Class Trait (Self : Set) : Type := {
@@ -32,21 +32,6 @@ Module result_info.
       Notation.dot := VALUE;
     }.
   End IsResultTypeFallback.
-  
-  Module
-    Impl_ink_result_info_IsResultTypeFallback_for_ink_result_info_IsResultType_T.
-    Section
-      Impl_ink_result_info_IsResultTypeFallback_for_ink_result_info_IsResultType_T.
-      Context {T : Set}.
-      Definition Self := ink.result_info.IsResultType T.
-      
-      Global Instance I : ink.result_info.IsResultTypeFallback.Trait Self := {
-      }.
-    End
-      Impl_ink_result_info_IsResultTypeFallback_for_ink_result_info_IsResultType_T.
-    Global Hint Resolve I : core.
-  End
-    Impl_ink_result_info_IsResultTypeFallback_for_ink_result_info_IsResultType_T.
   
   Module IsResultErr.
     Section IsResultErr.
@@ -74,25 +59,10 @@ Module result_info.
       Notation.dot (self : ref Self) := (axiom : M (H := H') bool);
     }.
   End IsResultErrFallback.
-  
-  Module
-    Impl_ink_result_info_IsResultErrFallback_for_ink_result_info_IsResultErr_T.
-    Section
-      Impl_ink_result_info_IsResultErrFallback_for_ink_result_info_IsResultErr_T.
-      Context {T : Set}.
-      Definition Self := ink.result_info.IsResultErr T.
-      
-      Global Instance I : ink.result_info.IsResultErrFallback.Trait Self := {
-      }.
-    End
-      Impl_ink_result_info_IsResultErrFallback_for_ink_result_info_IsResultErr_T.
-    Global Hint Resolve I : core.
-  End
-    Impl_ink_result_info_IsResultErrFallback_for_ink_result_info_IsResultErr_T.
 End result_info.
 
-Module IsResultType.
-  Section IsResultType.
+(* Module IsResultType.
+  (* Section IsResultType.
     Context {T : Set}.
     Unset Primitive Projections.
     Record t : Set := {
@@ -106,9 +76,9 @@ Module IsResultType.
     Global Instance Get_AF_marker : Notation.DoubleColon t "marker" := {
       Notation.double_colon '(Build_t x0) := x0;
     }.
-  End IsResultType.
-End IsResultType.
-Definition IsResultType (T : Set) : Set := IsResultType.t (T := T).
+  End IsResultType. *)
+End IsResultType. *)
+
 
 Module IsResultTypeFallback.
   Class Trait (Self : Set) : Type := {
@@ -120,21 +90,6 @@ Module IsResultTypeFallback.
     Notation.dot := VALUE;
   }.
 End IsResultTypeFallback.
-
-Module
-  Impl_ink_result_info_IsResultTypeFallback_for_ink_result_info_IsResultType_T.
-  Section
-    Impl_ink_result_info_IsResultTypeFallback_for_ink_result_info_IsResultType_T.
-    Context {T : Set}.
-    Definition Self := ink.result_info.IsResultType T.
-    
-    Global Instance I : ink.result_info.IsResultTypeFallback.Trait Self := {
-    }.
-  End
-    Impl_ink_result_info_IsResultTypeFallback_for_ink_result_info_IsResultType_T.
-  Global Hint Resolve I : core.
-End
-  Impl_ink_result_info_IsResultTypeFallback_for_ink_result_info_IsResultType_T.
 
 Module IsResultErr.
   Section IsResultErr.
@@ -162,20 +117,6 @@ Module IsResultErrFallback.
     Notation.dot (self : ref Self) := (axiom : M (H := H') bool);
   }.
 End IsResultErrFallback.
-
-Module
-  Impl_ink_result_info_IsResultErrFallback_for_ink_result_info_IsResultErr_T.
-  Section
-    Impl_ink_result_info_IsResultErrFallback_for_ink_result_info_IsResultErr_T.
-    Context {T : Set}.
-    Definition Self := ink.result_info.IsResultErr T.
-    
-    Global Instance I : ink.result_info.IsResultErrFallback.Trait Self := {
-    }.
-  End
-    Impl_ink_result_info_IsResultErrFallback_for_ink_result_info_IsResultErr_T.
-  Global Hint Resolve I : core.
-End Impl_ink_result_info_IsResultErrFallback_for_ink_result_info_IsResultErr_T.
 
 Module reflect.
   Module contract.
@@ -343,91 +284,6 @@ Module reflect.
     End ConstructorOutputValue.
     Definition ConstructorOutputValue := @ConstructorOutputValue.t.
     
-    Module
-      Impl_ink_reflect_dispatch_private_Sealed_for_ink_reflect_dispatch_ConstructorOutputValue_T.
-      Section
-        Impl_ink_reflect_dispatch_private_Sealed_for_ink_reflect_dispatch_ConstructorOutputValue_T.
-        Context {T : Set}.
-        Definition Self := ink.reflect.dispatch.ConstructorOutputValue T.
-        
-        Global Instance I : ink.reflect.dispatch.private.Sealed.Trait Self := {
-        }.
-      End
-        Impl_ink_reflect_dispatch_private_Sealed_for_ink_reflect_dispatch_ConstructorOutputValue_T.
-      Global Hint Resolve I : core.
-    End
-      Impl_ink_reflect_dispatch_private_Sealed_for_ink_reflect_dispatch_ConstructorOutputValue_T.
-    
-    Module
-      Impl_ink_reflect_dispatch_ConstructorOutput_for_ink_reflect_dispatch_ConstructorOutputValue_C.
-      Section
-        Impl_ink_reflect_dispatch_ConstructorOutput_for_ink_reflect_dispatch_ConstructorOutputValue_C.
-        Context {C : Set}.
-        Definition Self := ink.reflect.dispatch.ConstructorOutputValue C.
-        
-        Definition Error : Set := ref unit.
-        
-        Parameter as_result :
-            forall `{H' : State.Trait},
-            (ref Self) -> M (H := H') (core.result.Result (ref C) (ref Error)).
-        
-        Global Instance Method_as_result `{H' : State.Trait} :
-          Notation.Dot "as_result" := {
-          Notation.dot := as_result;
-        }.
-        
-        Global Instance I
-          : ink.reflect.dispatch.ConstructorOutput.Trait Self (C := C) := {
-          ink.reflect.dispatch.ConstructorOutput.Error := Error;
-          ink.reflect.dispatch.ConstructorOutput.as_result `{H' : State.Trait}
-            :=
-            as_result;
-        }.
-      End
-        Impl_ink_reflect_dispatch_ConstructorOutput_for_ink_reflect_dispatch_ConstructorOutputValue_C.
-      Global Hint Resolve I : core.
-    End
-      Impl_ink_reflect_dispatch_ConstructorOutput_for_ink_reflect_dispatch_ConstructorOutputValue_C.
-    
-    Module
-      Impl_ink_reflect_dispatch_ConstructorOutput_for_ink_reflect_dispatch_ConstructorOutputValue_core_result_Result_C_E.
-      Section
-        Impl_ink_reflect_dispatch_ConstructorOutput_for_ink_reflect_dispatch_ConstructorOutputValue_core_result_Result_C_E.
-        Context {C E : Set}.
-        Definition Self :=
-          ink.reflect.dispatch.ConstructorOutputValue (core.result.Result C E).
-        
-        Definition IS_RESULT `{H' : State.Trait} := Pure true.
-        
-        Global Instance AssociatedFunction_IS_RESULT `{H' : State.Trait} :
-          Notation.DoubleColon Self "IS_RESULT" := {
-          Notation.double_colon := IS_RESULT;
-        }.
-        
-        Definition Error : Set := E.
-        
-        Parameter as_result :
-            forall `{H' : State.Trait},
-            (ref Self) -> M (H := H') (core.result.Result (ref C) (ref Error)).
-        
-        Global Instance Method_as_result `{H' : State.Trait} :
-          Notation.Dot "as_result" := {
-          Notation.dot := as_result;
-        }.
-        
-        Global Instance I
-          : ink.reflect.dispatch.ConstructorOutput.Trait Self (C := C) := {
-          ink.reflect.dispatch.ConstructorOutput.Error := Error;
-          ink.reflect.dispatch.ConstructorOutput.as_result `{H' : State.Trait}
-            :=
-            as_result;
-        }.
-      End
-        Impl_ink_reflect_dispatch_ConstructorOutput_for_ink_reflect_dispatch_ConstructorOutputValue_core_result_Result_C_E.
-      Global Hint Resolve I : core.
-    End
-      Impl_ink_reflect_dispatch_ConstructorOutput_for_ink_reflect_dispatch_ConstructorOutputValue_core_result_Result_C_E.
-    
     Module DispatchError.
       Inductive t : Set :=
       | InvalidSelector
@@ -507,147 +363,6 @@ Module reflect.
         Notation.double_colon_type := Type_;
       }.
     End ContractConstructorDecoder.
-    
-    Module Impl_core_fmt_Debug_for_ink_reflect_dispatch_DispatchError.
-      Definition Self := ink.reflect.dispatch.DispatchError.
-      
-      Parameter fmt :
-          forall `{H' : State.Trait},
-          (ref Self) ->
-            (mut_ref core.fmt.Formatter) ->
-            M (H := H') core.fmt.Result.
-      
-      Global Instance Method_fmt `{H' : State.Trait} : Notation.Dot "fmt" := {
-        Notation.dot := fmt;
-      }.
-      
-      Global Instance I : core.fmt.Debug.Trait Self := {
-        core.fmt.Debug.fmt `{H' : State.Trait} := fmt;
-      }.
-      Global Hint Resolve I : core.
-    End Impl_core_fmt_Debug_for_ink_reflect_dispatch_DispatchError.
-    
-    Module Impl_core_marker_Copy_for_ink_reflect_dispatch_DispatchError.
-      Definition Self := ink.reflect.dispatch.DispatchError.
-      
-      Global Instance I : core.marker.Copy.Trait Self := {
-      }.
-      Global Hint Resolve I : core.
-    End Impl_core_marker_Copy_for_ink_reflect_dispatch_DispatchError.
-    
-    Module Impl_core_clone_Clone_for_ink_reflect_dispatch_DispatchError.
-      Definition Self := ink.reflect.dispatch.DispatchError.
-      
-      Parameter clone :
-          forall `{H' : State.Trait},
-          (ref Self) -> M (H := H') ink.reflect.dispatch.DispatchError.
-      
-      Global Instance Method_clone `{H' : State.Trait} :
-        Notation.Dot "clone" := {
-        Notation.dot := clone;
-      }.
-      
-      Global Instance I : core.clone.Clone.Trait Self := {
-        core.clone.Clone.clone `{H' : State.Trait} := clone;
-      }.
-      Global Hint Resolve I : core.
-    End Impl_core_clone_Clone_for_ink_reflect_dispatch_DispatchError.
-    
-    Module
-      Impl_core_marker_StructuralPartialEq_for_ink_reflect_dispatch_DispatchError.
-      Definition Self := ink.reflect.dispatch.DispatchError.
-      
-      Global Instance I : core.marker.StructuralPartialEq.Trait Self := {
-      }.
-      Global Hint Resolve I : core.
-    End
-      Impl_core_marker_StructuralPartialEq_for_ink_reflect_dispatch_DispatchError.
-    
-    Module Impl_core_cmp_PartialEq_for_ink_reflect_dispatch_DispatchError.
-      Definition Self := ink.reflect.dispatch.DispatchError.
-      
-      Parameter eq :
-          forall `{H' : State.Trait},
-          (ref Self) ->
-            (ref ink.reflect.dispatch.DispatchError) ->
-            M (H := H') bool.
-      
-      Global Instance Method_eq `{H' : State.Trait} : Notation.Dot "eq" := {
-        Notation.dot := eq;
-      }.
-      
-      Global Instance I
-        : core.cmp.PartialEq.Trait Self
-            (Rhs := core.cmp.PartialEq.Default.Rhs Self)
-          := {
-        core.cmp.PartialEq.eq `{H' : State.Trait} := eq;
-      }.
-      Global Hint Resolve I : core.
-    End Impl_core_cmp_PartialEq_for_ink_reflect_dispatch_DispatchError.
-    
-    Module Impl_core_marker_StructuralEq_for_ink_reflect_dispatch_DispatchError.
-      Definition Self := ink.reflect.dispatch.DispatchError.
-      
-      Global Instance I : core.marker.StructuralEq.Trait Self := {
-      }.
-      Global Hint Resolve I : core.
-    End Impl_core_marker_StructuralEq_for_ink_reflect_dispatch_DispatchError.
-    
-    Module Impl_core_cmp_Eq_for_ink_reflect_dispatch_DispatchError.
-      Definition Self := ink.reflect.dispatch.DispatchError.
-      
-      Parameter assert_receiver_is_total_eq :
-          forall `{H' : State.Trait},
-          (ref Self) -> M (H := H') unit.
-      
-      Global Instance Method_assert_receiver_is_total_eq `{H' : State.Trait} :
-        Notation.Dot "assert_receiver_is_total_eq" := {
-        Notation.dot := assert_receiver_is_total_eq;
-      }.
-      
-      Global Instance I : core.cmp.Eq.Trait Self := {
-      }.
-      Global Hint Resolve I : core.
-    End Impl_core_cmp_Eq_for_ink_reflect_dispatch_DispatchError.
-    
-    Module Impl_core_fmt_Display_for_ink_reflect_dispatch_DispatchError.
-      Definition Self := ink.reflect.dispatch.DispatchError.
-      
-      Parameter fmt :
-          forall `{H' : State.Trait},
-          (ref Self) ->
-            (mut_ref core.fmt.Formatter) ->
-            M (H := H') core.fmt.Result.
-      
-      Global Instance Method_fmt `{H' : State.Trait} : Notation.Dot "fmt" := {
-        Notation.dot := fmt;
-      }.
-      
-      Global Instance I : core.fmt.Display.Trait Self := {
-        core.fmt.Display.fmt `{H' : State.Trait} := fmt;
-      }.
-      Global Hint Resolve I : core.
-    End Impl_core_fmt_Display_for_ink_reflect_dispatch_DispatchError.
-    
-    Module Impl_core_convert_From_for_parity_scale_codec_error_Error.
-      Definition Self := parity_scale_codec.error.Error.
-      
-      Parameter from :
-          forall `{H' : State.Trait},
-          ink.reflect.dispatch.DispatchError -> M (H := H') Self.
-      
-      Global Instance AssociatedFunction_from `{H' : State.Trait} :
-        Notation.DoubleColon Self "from" := {
-        Notation.double_colon := from;
-      }.
-      
-      Global Instance I
-        : core.convert.From.Trait Self (T := ink.reflect.dispatch.DispatchError)
-          := {
-        core.convert.From.from `{H' : State.Trait} := from;
-      }.
-      Global Hint Resolve I : core.
-    End Impl_core_convert_From_for_parity_scale_codec_error_Error.
   End dispatch.
   
   Module event.
@@ -723,25 +438,6 @@ Module reflect.
       End TraitDefinitionRegistry.
       Definition TraitDefinitionRegistry (E : Set) : Set :=
         TraitDefinitionRegistry.t (E := E).
-      
-      Module
-        Impl_ink_env_contract_ContractEnv_for_ink_reflect_trait_def_registry_TraitDefinitionRegistry_E.
-        Section
-          Impl_ink_env_contract_ContractEnv_for_ink_reflect_trait_def_registry_TraitDefinitionRegistry_E.
-          Context {E : Set}.
-          Definition Self :=
-            ink.reflect.trait_def.registry.TraitDefinitionRegistry E.
-          
-          Definition Env : Set := E.
-          
-          Global Instance I : ink_env.contract.ContractEnv.Trait Self := {
-            ink_env.contract.ContractEnv.Env := Env;
-          }.
-        End
-          Impl_ink_env_contract_ContractEnv_for_ink_reflect_trait_def_registry_TraitDefinitionRegistry_E.
-        Global Hint Resolve I : core.
-      End
-        Impl_ink_env_contract_ContractEnv_for_ink_reflect_trait_def_registry_TraitDefinitionRegistry_E.
     End registry.
   End trait_def.
 End reflect.
@@ -927,17 +623,6 @@ Module codegen.
         Inductive t : Set := Build.
       End EventTopics.
       Definition EventTopics := @EventTopics.t.
-      
-      Module
-        Impl_ink_codegen_event_topics_RespectTopicLimit_for_ink_codegen_event_topics_EventTopics.
-        Definition Self := ink.codegen.event.topics.EventTopics.
-        
-        Global Instance I
-          : ink.codegen.event.topics.RespectTopicLimit.Trait Self := {
-        }.
-        Global Hint Resolve I : core.
-      End
-        Impl_ink_codegen_event_topics_RespectTopicLimit_for_ink_codegen_event_topics_EventTopics.
     End topics.
   End event.
   
@@ -948,62 +633,6 @@ Module codegen.
       }.
       Global Set Primitive Projections.
     End ImpliesReturn.
-    
-    Module Impl_ink_codegen_implies_return_ImpliesReturn_for_T.
-      Section Impl_ink_codegen_implies_return_ImpliesReturn_for_T.
-        Context {T : Set}.
-        Definition Self := T.
-        
-        Global Instance I
-          : ink.codegen.implies_return.ImpliesReturn.Trait Self (T := T) := {
-        }.
-      End Impl_ink_codegen_implies_return_ImpliesReturn_for_T.
-      Global Hint Resolve I : core.
-    End Impl_ink_codegen_implies_return_ImpliesReturn_for_T.
-    
-    Module
-      Impl_ink_codegen_implies_return_ImpliesReturn_for_ink_env_backend_and_call_builder_and_engine_and_engine_test_api_and_error_CallBuilder_E_ink_env_call_common_Set__CallType_ink_env_call_common_Set__ink_env_call_execution_input_ExecutionInput_Args_ink_env_call_common_Set__ink_env_call_common_ReturnType_T.
-      Section
-        Impl_ink_codegen_implies_return_ImpliesReturn_for_ink_env_backend_and_call_builder_and_engine_and_engine_test_api_and_error_CallBuilder_E_ink_env_call_common_Set__CallType_ink_env_call_common_Set__ink_env_call_execution_input_ExecutionInput_Args_ink_env_call_common_Set__ink_env_call_common_ReturnType_T.
-        Context {T E CallType Args : Set}.
-        Definition Self :=
-          ink_env.backend_and_call_builder_and_engine_and_engine_test_api_and_error.CallBuilder
-            E
-            (ink_env.call.common.Set_ CallType)
-            (ink_env.call.common.Set_
-              (ink_env.call.execution_input.ExecutionInput Args))
-            (ink_env.call.common.Set_ (ink_env.call.common.ReturnType T)).
-        
-        Global Instance I
-          : ink.codegen.implies_return.ImpliesReturn.Trait Self (T := T) := {
-        }.
-      End
-        Impl_ink_codegen_implies_return_ImpliesReturn_for_ink_env_backend_and_call_builder_and_engine_and_engine_test_api_and_error_CallBuilder_E_ink_env_call_common_Set__CallType_ink_env_call_common_Set__ink_env_call_execution_input_ExecutionInput_Args_ink_env_call_common_Set__ink_env_call_common_ReturnType_T.
-      Global Hint Resolve I : core.
-    End
-      Impl_ink_codegen_implies_return_ImpliesReturn_for_ink_env_backend_and_call_builder_and_engine_and_engine_test_api_and_error_CallBuilder_E_ink_env_call_common_Set__CallType_ink_env_call_common_Set__ink_env_call_execution_input_ExecutionInput_Args_ink_env_call_common_Set__ink_env_call_common_ReturnType_T.
-    
-    Module
-      Impl_ink_codegen_implies_return_ImpliesReturn_for_ink_env_backend_and_call_builder_and_engine_and_engine_test_api_and_error_CallBuilder_E_ink_env_call_common_Set__CallType_ink_env_call_common_Set__ink_env_call_execution_input_ExecutionInput_Args_ink_env_call_common_Set__Tuple_.
-      Section
-        Impl_ink_codegen_implies_return_ImpliesReturn_for_ink_env_backend_and_call_builder_and_engine_and_engine_test_api_and_error_CallBuilder_E_ink_env_call_common_Set__CallType_ink_env_call_common_Set__ink_env_call_execution_input_ExecutionInput_Args_ink_env_call_common_Set__Tuple_.
-        Context {E CallType Args : Set}.
-        Definition Self :=
-          ink_env.backend_and_call_builder_and_engine_and_engine_test_api_and_error.CallBuilder
-            E
-            (ink_env.call.common.Set_ CallType)
-            (ink_env.call.common.Set_
-              (ink_env.call.execution_input.ExecutionInput Args))
-            (ink_env.call.common.Set_ unit).
-        
-        Global Instance I
-          : ink.codegen.implies_return.ImpliesReturn.Trait Self (T := unit) := {
-        }.
-      End
-        Impl_ink_codegen_implies_return_ImpliesReturn_for_ink_env_backend_and_call_builder_and_engine_and_engine_test_api_and_error_CallBuilder_E_ink_env_call_common_Set__CallType_ink_env_call_common_Set__ink_env_call_execution_input_ExecutionInput_Args_ink_env_call_common_Set__Tuple_.
-      Global Hint Resolve I : core.
-    End
-      Impl_ink_codegen_implies_return_ImpliesReturn_for_ink_env_backend_and_call_builder_and_engine_and_engine_test_api_and_error_CallBuilder_E_ink_env_call_common_Set__CallType_ink_env_call_common_Set__ink_env_call_execution_input_ExecutionInput_Args_ink_env_call_common_Set__Tuple_.
   End implies_return.
   
   Module trait_def.
@@ -1457,17 +1086,6 @@ Module event.
       Inductive t : Set := Build.
     End EventTopics.
     Definition EventTopics := @EventTopics.t.
-    
-    Module
-      Impl_ink_codegen_event_topics_RespectTopicLimit_for_ink_codegen_event_topics_EventTopics.
-      Definition Self := ink.codegen.event.topics.EventTopics.
-      
-      Global Instance I
-        : ink.codegen.event.topics.RespectTopicLimit.Trait Self := {
-      }.
-      Global Hint Resolve I : core.
-    End
-      Impl_ink_codegen_event_topics_RespectTopicLimit_for_ink_codegen_event_topics_EventTopics.
   End topics.
 End event.
 
@@ -1586,17 +1204,6 @@ Module topics.
     Inductive t : Set := Build.
   End EventTopics.
   Definition EventTopics := @EventTopics.t.
-  
-  Module
-    Impl_ink_codegen_event_topics_RespectTopicLimit_for_ink_codegen_event_topics_EventTopics.
-    Definition Self := ink.codegen.event.topics.EventTopics.
-    
-    Global Instance I
-      : ink.codegen.event.topics.RespectTopicLimit.Trait Self := {
-    }.
-    Global Hint Resolve I : core.
-  End
-    Impl_ink_codegen_event_topics_RespectTopicLimit_for_ink_codegen_event_topics_EventTopics.
 End topics.
 
 Module EventRespectsTopicLimit.
@@ -1641,16 +1248,6 @@ Module EventTopics.
 End EventTopics.
 Definition EventTopics := @EventTopics.t.
 
-Module
-  Impl_ink_codegen_event_topics_RespectTopicLimit_for_ink_codegen_event_topics_EventTopics.
-  Definition Self := ink.codegen.event.topics.EventTopics.
-  
-  Global Instance I : ink.codegen.event.topics.RespectTopicLimit.Trait Self := {
-  }.
-  Global Hint Resolve I : core.
-End
-  Impl_ink_codegen_event_topics_RespectTopicLimit_for_ink_codegen_event_topics_EventTopics.
-
 Module EventLenTopics.
   Class Trait (Self : Set) : Type := {
     LenTopics : Set;
@@ -1669,62 +1266,6 @@ Module implies_return.
     }.
     Global Set Primitive Projections.
   End ImpliesReturn.
-  
-  Module Impl_ink_codegen_implies_return_ImpliesReturn_for_T.
-    Section Impl_ink_codegen_implies_return_ImpliesReturn_for_T.
-      Context {T : Set}.
-      Definition Self := T.
-      
-      Global Instance I
-        : ink.codegen.implies_return.ImpliesReturn.Trait Self (T := T) := {
-      }.
-    End Impl_ink_codegen_implies_return_ImpliesReturn_for_T.
-    Global Hint Resolve I : core.
-  End Impl_ink_codegen_implies_return_ImpliesReturn_for_T.
-  
-  Module
-    Impl_ink_codegen_implies_return_ImpliesReturn_for_ink_env_backend_and_call_builder_and_engine_and_engine_test_api_and_error_CallBuilder_E_ink_env_call_common_Set__CallType_ink_env_call_common_Set__ink_env_call_execution_input_ExecutionInput_Args_ink_env_call_common_Set__ink_env_call_common_ReturnType_T.
-    Section
-      Impl_ink_codegen_implies_return_ImpliesReturn_for_ink_env_backend_and_call_builder_and_engine_and_engine_test_api_and_error_CallBuilder_E_ink_env_call_common_Set__CallType_ink_env_call_common_Set__ink_env_call_execution_input_ExecutionInput_Args_ink_env_call_common_Set__ink_env_call_common_ReturnType_T.
-      Context {T E CallType Args : Set}.
-      Definition Self :=
-        ink_env.backend_and_call_builder_and_engine_and_engine_test_api_and_error.CallBuilder
-          E
-          (ink_env.call.common.Set_ CallType)
-          (ink_env.call.common.Set_
-            (ink_env.call.execution_input.ExecutionInput Args))
-          (ink_env.call.common.Set_ (ink_env.call.common.ReturnType T)).
-      
-      Global Instance I
-        : ink.codegen.implies_return.ImpliesReturn.Trait Self (T := T) := {
-      }.
-    End
-      Impl_ink_codegen_implies_return_ImpliesReturn_for_ink_env_backend_and_call_builder_and_engine_and_engine_test_api_and_error_CallBuilder_E_ink_env_call_common_Set__CallType_ink_env_call_common_Set__ink_env_call_execution_input_ExecutionInput_Args_ink_env_call_common_Set__ink_env_call_common_ReturnType_T.
-    Global Hint Resolve I : core.
-  End
-    Impl_ink_codegen_implies_return_ImpliesReturn_for_ink_env_backend_and_call_builder_and_engine_and_engine_test_api_and_error_CallBuilder_E_ink_env_call_common_Set__CallType_ink_env_call_common_Set__ink_env_call_execution_input_ExecutionInput_Args_ink_env_call_common_Set__ink_env_call_common_ReturnType_T.
-  
-  Module
-    Impl_ink_codegen_implies_return_ImpliesReturn_for_ink_env_backend_and_call_builder_and_engine_and_engine_test_api_and_error_CallBuilder_E_ink_env_call_common_Set__CallType_ink_env_call_common_Set__ink_env_call_execution_input_ExecutionInput_Args_ink_env_call_common_Set__Tuple_.
-    Section
-      Impl_ink_codegen_implies_return_ImpliesReturn_for_ink_env_backend_and_call_builder_and_engine_and_engine_test_api_and_error_CallBuilder_E_ink_env_call_common_Set__CallType_ink_env_call_common_Set__ink_env_call_execution_input_ExecutionInput_Args_ink_env_call_common_Set__Tuple_.
-      Context {E CallType Args : Set}.
-      Definition Self :=
-        ink_env.backend_and_call_builder_and_engine_and_engine_test_api_and_error.CallBuilder
-          E
-          (ink_env.call.common.Set_ CallType)
-          (ink_env.call.common.Set_
-            (ink_env.call.execution_input.ExecutionInput Args))
-          (ink_env.call.common.Set_ unit).
-      
-      Global Instance I
-        : ink.codegen.implies_return.ImpliesReturn.Trait Self (T := unit) := {
-      }.
-    End
-      Impl_ink_codegen_implies_return_ImpliesReturn_for_ink_env_backend_and_call_builder_and_engine_and_engine_test_api_and_error_CallBuilder_E_ink_env_call_common_Set__CallType_ink_env_call_common_Set__ink_env_call_execution_input_ExecutionInput_Args_ink_env_call_common_Set__Tuple_.
-    Global Hint Resolve I : core.
-  End
-    Impl_ink_codegen_implies_return_ImpliesReturn_for_ink_env_backend_and_call_builder_and_engine_and_engine_test_api_and_error_CallBuilder_E_ink_env_call_common_Set__CallType_ink_env_call_common_Set__ink_env_call_execution_input_ExecutionInput_Args_ink_env_call_common_Set__Tuple_.
 End implies_return.
 
 Module ImpliesReturn.
@@ -1733,62 +1274,6 @@ Module ImpliesReturn.
   }.
   Global Set Primitive Projections.
 End ImpliesReturn.
-
-Module Impl_ink_codegen_implies_return_ImpliesReturn_for_T.
-  Section Impl_ink_codegen_implies_return_ImpliesReturn_for_T.
-    Context {T : Set}.
-    Definition Self := T.
-    
-    Global Instance I
-      : ink.codegen.implies_return.ImpliesReturn.Trait Self (T := T) := {
-    }.
-  End Impl_ink_codegen_implies_return_ImpliesReturn_for_T.
-  Global Hint Resolve I : core.
-End Impl_ink_codegen_implies_return_ImpliesReturn_for_T.
-
-Module
-  Impl_ink_codegen_implies_return_ImpliesReturn_for_ink_env_backend_and_call_builder_and_engine_and_engine_test_api_and_error_CallBuilder_E_ink_env_call_common_Set__CallType_ink_env_call_common_Set__ink_env_call_execution_input_ExecutionInput_Args_ink_env_call_common_Set__ink_env_call_common_ReturnType_T.
-  Section
-    Impl_ink_codegen_implies_return_ImpliesReturn_for_ink_env_backend_and_call_builder_and_engine_and_engine_test_api_and_error_CallBuilder_E_ink_env_call_common_Set__CallType_ink_env_call_common_Set__ink_env_call_execution_input_ExecutionInput_Args_ink_env_call_common_Set__ink_env_call_common_ReturnType_T.
-    Context {T E CallType Args : Set}.
-    Definition Self :=
-      ink_env.backend_and_call_builder_and_engine_and_engine_test_api_and_error.CallBuilder
-        E
-        (ink_env.call.common.Set_ CallType)
-        (ink_env.call.common.Set_
-          (ink_env.call.execution_input.ExecutionInput Args))
-        (ink_env.call.common.Set_ (ink_env.call.common.ReturnType T)).
-    
-    Global Instance I
-      : ink.codegen.implies_return.ImpliesReturn.Trait Self (T := T) := {
-    }.
-  End
-    Impl_ink_codegen_implies_return_ImpliesReturn_for_ink_env_backend_and_call_builder_and_engine_and_engine_test_api_and_error_CallBuilder_E_ink_env_call_common_Set__CallType_ink_env_call_common_Set__ink_env_call_execution_input_ExecutionInput_Args_ink_env_call_common_Set__ink_env_call_common_ReturnType_T.
-  Global Hint Resolve I : core.
-End
-  Impl_ink_codegen_implies_return_ImpliesReturn_for_ink_env_backend_and_call_builder_and_engine_and_engine_test_api_and_error_CallBuilder_E_ink_env_call_common_Set__CallType_ink_env_call_common_Set__ink_env_call_execution_input_ExecutionInput_Args_ink_env_call_common_Set__ink_env_call_common_ReturnType_T.
-
-Module
-  Impl_ink_codegen_implies_return_ImpliesReturn_for_ink_env_backend_and_call_builder_and_engine_and_engine_test_api_and_error_CallBuilder_E_ink_env_call_common_Set__CallType_ink_env_call_common_Set__ink_env_call_execution_input_ExecutionInput_Args_ink_env_call_common_Set__Tuple_.
-  Section
-    Impl_ink_codegen_implies_return_ImpliesReturn_for_ink_env_backend_and_call_builder_and_engine_and_engine_test_api_and_error_CallBuilder_E_ink_env_call_common_Set__CallType_ink_env_call_common_Set__ink_env_call_execution_input_ExecutionInput_Args_ink_env_call_common_Set__Tuple_.
-    Context {E CallType Args : Set}.
-    Definition Self :=
-      ink_env.backend_and_call_builder_and_engine_and_engine_test_api_and_error.CallBuilder
-        E
-        (ink_env.call.common.Set_ CallType)
-        (ink_env.call.common.Set_
-          (ink_env.call.execution_input.ExecutionInput Args))
-        (ink_env.call.common.Set_ unit).
-    
-    Global Instance I
-      : ink.codegen.implies_return.ImpliesReturn.Trait Self (T := unit) := {
-    }.
-  End
-    Impl_ink_codegen_implies_return_ImpliesReturn_for_ink_env_backend_and_call_builder_and_engine_and_engine_test_api_and_error_CallBuilder_E_ink_env_call_common_Set__CallType_ink_env_call_common_Set__ink_env_call_execution_input_ExecutionInput_Args_ink_env_call_common_Set__Tuple_.
-  Global Hint Resolve I : core.
-End
-  Impl_ink_codegen_implies_return_ImpliesReturn_for_ink_env_backend_and_call_builder_and_engine_and_engine_test_api_and_error_CallBuilder_E_ink_env_call_common_Set__CallType_ink_env_call_common_Set__ink_env_call_execution_input_ExecutionInput_Args_ink_env_call_common_Set__Tuple_.
 
 Module trait_def.
   Module call_builder.
@@ -2355,91 +1840,6 @@ Module Wrap_dispatch_1.
     End ConstructorOutputValue.
     Definition ConstructorOutputValue := @ConstructorOutputValue.t.
     
-    Module
-      Impl_ink_reflect_dispatch_private_Sealed_for_ink_reflect_dispatch_ConstructorOutputValue_T.
-      Section
-        Impl_ink_reflect_dispatch_private_Sealed_for_ink_reflect_dispatch_ConstructorOutputValue_T.
-        Context {T : Set}.
-        Definition Self := ink.reflect.dispatch.ConstructorOutputValue T.
-        
-        Global Instance I : ink.reflect.dispatch.private.Sealed.Trait Self := {
-        }.
-      End
-        Impl_ink_reflect_dispatch_private_Sealed_for_ink_reflect_dispatch_ConstructorOutputValue_T.
-      Global Hint Resolve I : core.
-    End
-      Impl_ink_reflect_dispatch_private_Sealed_for_ink_reflect_dispatch_ConstructorOutputValue_T.
-    
-    Module
-      Impl_ink_reflect_dispatch_ConstructorOutput_for_ink_reflect_dispatch_ConstructorOutputValue_C.
-      Section
-        Impl_ink_reflect_dispatch_ConstructorOutput_for_ink_reflect_dispatch_ConstructorOutputValue_C.
-        Context {C : Set}.
-        Definition Self := ink.reflect.dispatch.ConstructorOutputValue C.
-        
-        Definition Error : Set := ref unit.
-        
-        Parameter as_result :
-            forall `{H' : State.Trait},
-            (ref Self) -> M (H := H') (core.result.Result (ref C) (ref Error)).
-        
-        Global Instance Method_as_result `{H' : State.Trait} :
-          Notation.Dot "as_result" := {
-          Notation.dot := as_result;
-        }.
-        
-        Global Instance I
-          : ink.reflect.dispatch.ConstructorOutput.Trait Self (C := C) := {
-          ink.reflect.dispatch.ConstructorOutput.Error := Error;
-          ink.reflect.dispatch.ConstructorOutput.as_result `{H' : State.Trait}
-            :=
-            as_result;
-        }.
-      End
-        Impl_ink_reflect_dispatch_ConstructorOutput_for_ink_reflect_dispatch_ConstructorOutputValue_C.
-      Global Hint Resolve I : core.
-    End
-      Impl_ink_reflect_dispatch_ConstructorOutput_for_ink_reflect_dispatch_ConstructorOutputValue_C.
-    
-    Module
-      Impl_ink_reflect_dispatch_ConstructorOutput_for_ink_reflect_dispatch_ConstructorOutputValue_core_result_Result_C_E.
-      Section
-        Impl_ink_reflect_dispatch_ConstructorOutput_for_ink_reflect_dispatch_ConstructorOutputValue_core_result_Result_C_E.
-        Context {C E : Set}.
-        Definition Self :=
-          ink.reflect.dispatch.ConstructorOutputValue (core.result.Result C E).
-        
-        Definition IS_RESULT `{H' : State.Trait} := Pure true.
-        
-        Global Instance AssociatedFunction_IS_RESULT `{H' : State.Trait} :
-          Notation.DoubleColon Self "IS_RESULT" := {
-          Notation.double_colon := IS_RESULT;
-        }.
-        
-        Definition Error : Set := E.
-        
-        Parameter as_result :
-            forall `{H' : State.Trait},
-            (ref Self) -> M (H := H') (core.result.Result (ref C) (ref Error)).
-        
-        Global Instance Method_as_result `{H' : State.Trait} :
-          Notation.Dot "as_result" := {
-          Notation.dot := as_result;
-        }.
-        
-        Global Instance I
-          : ink.reflect.dispatch.ConstructorOutput.Trait Self (C := C) := {
-          ink.reflect.dispatch.ConstructorOutput.Error := Error;
-          ink.reflect.dispatch.ConstructorOutput.as_result `{H' : State.Trait}
-            :=
-            as_result;
-        }.
-      End
-        Impl_ink_reflect_dispatch_ConstructorOutput_for_ink_reflect_dispatch_ConstructorOutputValue_core_result_Result_C_E.
-      Global Hint Resolve I : core.
-    End
-      Impl_ink_reflect_dispatch_ConstructorOutput_for_ink_reflect_dispatch_ConstructorOutputValue_core_result_Result_C_E.
-    
     Module DispatchError.
       Inductive t : Set :=
       | InvalidSelector
@@ -2519,147 +1919,6 @@ Module Wrap_dispatch_1.
         Notation.double_colon_type := Type_;
       }.
     End ContractConstructorDecoder.
-    
-    Module Impl_core_fmt_Debug_for_ink_reflect_dispatch_DispatchError.
-      Definition Self := ink.reflect.dispatch.DispatchError.
-      
-      Parameter fmt :
-          forall `{H' : State.Trait},
-          (ref Self) ->
-            (mut_ref core.fmt.Formatter) ->
-            M (H := H') core.fmt.Result.
-      
-      Global Instance Method_fmt `{H' : State.Trait} : Notation.Dot "fmt" := {
-        Notation.dot := fmt;
-      }.
-      
-      Global Instance I : core.fmt.Debug.Trait Self := {
-        core.fmt.Debug.fmt `{H' : State.Trait} := fmt;
-      }.
-      Global Hint Resolve I : core.
-    End Impl_core_fmt_Debug_for_ink_reflect_dispatch_DispatchError.
-    
-    Module Impl_core_marker_Copy_for_ink_reflect_dispatch_DispatchError.
-      Definition Self := ink.reflect.dispatch.DispatchError.
-      
-      Global Instance I : core.marker.Copy.Trait Self := {
-      }.
-      Global Hint Resolve I : core.
-    End Impl_core_marker_Copy_for_ink_reflect_dispatch_DispatchError.
-    
-    Module Impl_core_clone_Clone_for_ink_reflect_dispatch_DispatchError.
-      Definition Self := ink.reflect.dispatch.DispatchError.
-      
-      Parameter clone :
-          forall `{H' : State.Trait},
-          (ref Self) -> M (H := H') ink.reflect.dispatch.DispatchError.
-      
-      Global Instance Method_clone `{H' : State.Trait} :
-        Notation.Dot "clone" := {
-        Notation.dot := clone;
-      }.
-      
-      Global Instance I : core.clone.Clone.Trait Self := {
-        core.clone.Clone.clone `{H' : State.Trait} := clone;
-      }.
-      Global Hint Resolve I : core.
-    End Impl_core_clone_Clone_for_ink_reflect_dispatch_DispatchError.
-    
-    Module
-      Impl_core_marker_StructuralPartialEq_for_ink_reflect_dispatch_DispatchError.
-      Definition Self := ink.reflect.dispatch.DispatchError.
-      
-      Global Instance I : core.marker.StructuralPartialEq.Trait Self := {
-      }.
-      Global Hint Resolve I : core.
-    End
-      Impl_core_marker_StructuralPartialEq_for_ink_reflect_dispatch_DispatchError.
-    
-    Module Impl_core_cmp_PartialEq_for_ink_reflect_dispatch_DispatchError.
-      Definition Self := ink.reflect.dispatch.DispatchError.
-      
-      Parameter eq :
-          forall `{H' : State.Trait},
-          (ref Self) ->
-            (ref ink.reflect.dispatch.DispatchError) ->
-            M (H := H') bool.
-      
-      Global Instance Method_eq `{H' : State.Trait} : Notation.Dot "eq" := {
-        Notation.dot := eq;
-      }.
-      
-      Global Instance I
-        : core.cmp.PartialEq.Trait Self
-            (Rhs := core.cmp.PartialEq.Default.Rhs Self)
-          := {
-        core.cmp.PartialEq.eq `{H' : State.Trait} := eq;
-      }.
-      Global Hint Resolve I : core.
-    End Impl_core_cmp_PartialEq_for_ink_reflect_dispatch_DispatchError.
-    
-    Module Impl_core_marker_StructuralEq_for_ink_reflect_dispatch_DispatchError.
-      Definition Self := ink.reflect.dispatch.DispatchError.
-      
-      Global Instance I : core.marker.StructuralEq.Trait Self := {
-      }.
-      Global Hint Resolve I : core.
-    End Impl_core_marker_StructuralEq_for_ink_reflect_dispatch_DispatchError.
-    
-    Module Impl_core_cmp_Eq_for_ink_reflect_dispatch_DispatchError.
-      Definition Self := ink.reflect.dispatch.DispatchError.
-      
-      Parameter assert_receiver_is_total_eq :
-          forall `{H' : State.Trait},
-          (ref Self) -> M (H := H') unit.
-      
-      Global Instance Method_assert_receiver_is_total_eq `{H' : State.Trait} :
-        Notation.Dot "assert_receiver_is_total_eq" := {
-        Notation.dot := assert_receiver_is_total_eq;
-      }.
-      
-      Global Instance I : core.cmp.Eq.Trait Self := {
-      }.
-      Global Hint Resolve I : core.
-    End Impl_core_cmp_Eq_for_ink_reflect_dispatch_DispatchError.
-    
-    Module Impl_core_fmt_Display_for_ink_reflect_dispatch_DispatchError.
-      Definition Self := ink.reflect.dispatch.DispatchError.
-      
-      Parameter fmt :
-          forall `{H' : State.Trait},
-          (ref Self) ->
-            (mut_ref core.fmt.Formatter) ->
-            M (H := H') core.fmt.Result.
-      
-      Global Instance Method_fmt `{H' : State.Trait} : Notation.Dot "fmt" := {
-        Notation.dot := fmt;
-      }.
-      
-      Global Instance I : core.fmt.Display.Trait Self := {
-        core.fmt.Display.fmt `{H' : State.Trait} := fmt;
-      }.
-      Global Hint Resolve I : core.
-    End Impl_core_fmt_Display_for_ink_reflect_dispatch_DispatchError.
-    
-    Module Impl_core_convert_From_for_parity_scale_codec_error_Error.
-      Definition Self := parity_scale_codec.error.Error.
-      
-      Parameter from :
-          forall `{H' : State.Trait},
-          ink.reflect.dispatch.DispatchError -> M (H := H') Self.
-      
-      Global Instance AssociatedFunction_from `{H' : State.Trait} :
-        Notation.DoubleColon Self "from" := {
-        Notation.double_colon := from;
-      }.
-      
-      Global Instance I
-        : core.convert.From.Trait Self (T := ink.reflect.dispatch.DispatchError)
-          := {
-        core.convert.From.from `{H' : State.Trait} := from;
-      }.
-      Global Hint Resolve I : core.
-    End Impl_core_convert_From_for_parity_scale_codec_error_Error.
   End dispatch.
 End Wrap_dispatch_1.
 Import Wrap_dispatch_1.
@@ -2822,91 +2081,6 @@ Module ConstructorOutputValue.
 End ConstructorOutputValue.
 Definition ConstructorOutputValue := @ConstructorOutputValue.t.
 
-Module
-  Impl_ink_reflect_dispatch_private_Sealed_for_ink_reflect_dispatch_ConstructorOutputValue_T.
-  Section
-    Impl_ink_reflect_dispatch_private_Sealed_for_ink_reflect_dispatch_ConstructorOutputValue_T.
-    Context {T : Set}.
-    Definition Self := ink.reflect.dispatch.ConstructorOutputValue T.
-    
-    Global Instance I : ink.reflect.dispatch.private.Sealed.Trait Self := {
-    }.
-  End
-    Impl_ink_reflect_dispatch_private_Sealed_for_ink_reflect_dispatch_ConstructorOutputValue_T.
-  Global Hint Resolve I : core.
-End
-  Impl_ink_reflect_dispatch_private_Sealed_for_ink_reflect_dispatch_ConstructorOutputValue_T.
-
-Module
-  Impl_ink_reflect_dispatch_ConstructorOutput_for_ink_reflect_dispatch_ConstructorOutputValue_C.
-  Section
-    Impl_ink_reflect_dispatch_ConstructorOutput_for_ink_reflect_dispatch_ConstructorOutputValue_C.
-    Context {C : Set}.
-    Definition Self := ink.reflect.dispatch.ConstructorOutputValue C.
-    
-    Definition Error : Set := ref unit.
-    
-    Parameter as_result :
-        forall `{H' : State.Trait},
-        (ref Self) -> M (H := H') (core.result.Result (ref C) (ref Error)).
-    
-    Global Instance Method_as_result `{H' : State.Trait} :
-      Notation.Dot "as_result" := {
-      Notation.dot := as_result;
-    }.
-    
-    Global Instance I
-      : ink.reflect.dispatch.ConstructorOutput.Trait Self (C := C) := {
-      ink.reflect.dispatch.ConstructorOutput.Error := Error;
-      ink.reflect.dispatch.ConstructorOutput.as_result `{H' : State.Trait}
-        :=
-        as_result;
-    }.
-  End
-    Impl_ink_reflect_dispatch_ConstructorOutput_for_ink_reflect_dispatch_ConstructorOutputValue_C.
-  Global Hint Resolve I : core.
-End
-  Impl_ink_reflect_dispatch_ConstructorOutput_for_ink_reflect_dispatch_ConstructorOutputValue_C.
-
-Module
-  Impl_ink_reflect_dispatch_ConstructorOutput_for_ink_reflect_dispatch_ConstructorOutputValue_core_result_Result_C_E.
-  Section
-    Impl_ink_reflect_dispatch_ConstructorOutput_for_ink_reflect_dispatch_ConstructorOutputValue_core_result_Result_C_E.
-    Context {C E : Set}.
-    Definition Self :=
-      ink.reflect.dispatch.ConstructorOutputValue (core.result.Result C E).
-    
-    Definition IS_RESULT `{H' : State.Trait} := Pure true.
-    
-    Global Instance AssociatedFunction_IS_RESULT `{H' : State.Trait} :
-      Notation.DoubleColon Self "IS_RESULT" := {
-      Notation.double_colon := IS_RESULT;
-    }.
-    
-    Definition Error : Set := E.
-    
-    Parameter as_result :
-        forall `{H' : State.Trait},
-        (ref Self) -> M (H := H') (core.result.Result (ref C) (ref Error)).
-    
-    Global Instance Method_as_result `{H' : State.Trait} :
-      Notation.Dot "as_result" := {
-      Notation.dot := as_result;
-    }.
-    
-    Global Instance I
-      : ink.reflect.dispatch.ConstructorOutput.Trait Self (C := C) := {
-      ink.reflect.dispatch.ConstructorOutput.Error := Error;
-      ink.reflect.dispatch.ConstructorOutput.as_result `{H' : State.Trait}
-        :=
-        as_result;
-    }.
-  End
-    Impl_ink_reflect_dispatch_ConstructorOutput_for_ink_reflect_dispatch_ConstructorOutputValue_core_result_Result_C_E.
-  Global Hint Resolve I : core.
-End
-  Impl_ink_reflect_dispatch_ConstructorOutput_for_ink_reflect_dispatch_ConstructorOutputValue_core_result_Result_C_E.
-
 Module ContractMessageDecoder.
   Class Trait (Self : Set) : Type := {
     Type_ : Set;
@@ -2965,140 +2139,6 @@ Module DispatchError.
   | PaidUnpayableMessage.
 End DispatchError.
 Definition DispatchError := DispatchError.t.
-
-Module Impl_core_fmt_Debug_for_ink_reflect_dispatch_DispatchError.
-  Definition Self := ink.reflect.dispatch.DispatchError.
-  
-  Parameter fmt :
-      forall `{H' : State.Trait},
-      (ref Self) -> (mut_ref core.fmt.Formatter) -> M (H := H') core.fmt.Result.
-  
-  Global Instance Method_fmt `{H' : State.Trait} : Notation.Dot "fmt" := {
-    Notation.dot := fmt;
-  }.
-  
-  Global Instance I : core.fmt.Debug.Trait Self := {
-    core.fmt.Debug.fmt `{H' : State.Trait} := fmt;
-  }.
-  Global Hint Resolve I : core.
-End Impl_core_fmt_Debug_for_ink_reflect_dispatch_DispatchError.
-
-Module Impl_core_marker_Copy_for_ink_reflect_dispatch_DispatchError.
-  Definition Self := ink.reflect.dispatch.DispatchError.
-  
-  Global Instance I : core.marker.Copy.Trait Self := {
-  }.
-  Global Hint Resolve I : core.
-End Impl_core_marker_Copy_for_ink_reflect_dispatch_DispatchError.
-
-Module Impl_core_clone_Clone_for_ink_reflect_dispatch_DispatchError.
-  Definition Self := ink.reflect.dispatch.DispatchError.
-  
-  Parameter clone :
-      forall `{H' : State.Trait},
-      (ref Self) -> M (H := H') ink.reflect.dispatch.DispatchError.
-  
-  Global Instance Method_clone `{H' : State.Trait} : Notation.Dot "clone" := {
-    Notation.dot := clone;
-  }.
-  
-  Global Instance I : core.clone.Clone.Trait Self := {
-    core.clone.Clone.clone `{H' : State.Trait} := clone;
-  }.
-  Global Hint Resolve I : core.
-End Impl_core_clone_Clone_for_ink_reflect_dispatch_DispatchError.
-
-Module
-  Impl_core_marker_StructuralPartialEq_for_ink_reflect_dispatch_DispatchError.
-  Definition Self := ink.reflect.dispatch.DispatchError.
-  
-  Global Instance I : core.marker.StructuralPartialEq.Trait Self := {
-  }.
-  Global Hint Resolve I : core.
-End Impl_core_marker_StructuralPartialEq_for_ink_reflect_dispatch_DispatchError.
-
-Module Impl_core_cmp_PartialEq_for_ink_reflect_dispatch_DispatchError.
-  Definition Self := ink.reflect.dispatch.DispatchError.
-  
-  Parameter eq :
-      forall `{H' : State.Trait},
-      (ref Self) ->
-        (ref ink.reflect.dispatch.DispatchError) ->
-        M (H := H') bool.
-  
-  Global Instance Method_eq `{H' : State.Trait} : Notation.Dot "eq" := {
-    Notation.dot := eq;
-  }.
-  
-  Global Instance I
-    : core.cmp.PartialEq.Trait Self (Rhs := core.cmp.PartialEq.Default.Rhs Self)
-      := {
-    core.cmp.PartialEq.eq `{H' : State.Trait} := eq;
-  }.
-  Global Hint Resolve I : core.
-End Impl_core_cmp_PartialEq_for_ink_reflect_dispatch_DispatchError.
-
-Module Impl_core_marker_StructuralEq_for_ink_reflect_dispatch_DispatchError.
-  Definition Self := ink.reflect.dispatch.DispatchError.
-  
-  Global Instance I : core.marker.StructuralEq.Trait Self := {
-  }.
-  Global Hint Resolve I : core.
-End Impl_core_marker_StructuralEq_for_ink_reflect_dispatch_DispatchError.
-
-Module Impl_core_cmp_Eq_for_ink_reflect_dispatch_DispatchError.
-  Definition Self := ink.reflect.dispatch.DispatchError.
-  
-  Parameter assert_receiver_is_total_eq :
-      forall `{H' : State.Trait},
-      (ref Self) -> M (H := H') unit.
-  
-  Global Instance Method_assert_receiver_is_total_eq `{H' : State.Trait} :
-    Notation.Dot "assert_receiver_is_total_eq" := {
-    Notation.dot := assert_receiver_is_total_eq;
-  }.
-  
-  Global Instance I : core.cmp.Eq.Trait Self := {
-  }.
-  Global Hint Resolve I : core.
-End Impl_core_cmp_Eq_for_ink_reflect_dispatch_DispatchError.
-
-Module Impl_core_fmt_Display_for_ink_reflect_dispatch_DispatchError.
-  Definition Self := ink.reflect.dispatch.DispatchError.
-  
-  Parameter fmt :
-      forall `{H' : State.Trait},
-      (ref Self) -> (mut_ref core.fmt.Formatter) -> M (H := H') core.fmt.Result.
-  
-  Global Instance Method_fmt `{H' : State.Trait} : Notation.Dot "fmt" := {
-    Notation.dot := fmt;
-  }.
-  
-  Global Instance I : core.fmt.Display.Trait Self := {
-    core.fmt.Display.fmt `{H' : State.Trait} := fmt;
-  }.
-  Global Hint Resolve I : core.
-End Impl_core_fmt_Display_for_ink_reflect_dispatch_DispatchError.
-
-Module Impl_core_convert_From_for_parity_scale_codec_error_Error.
-  Definition Self := parity_scale_codec.error.Error.
-  
-  Parameter from :
-      forall `{H' : State.Trait},
-      ink.reflect.dispatch.DispatchError -> M (H := H') Self.
-  
-  Global Instance AssociatedFunction_from `{H' : State.Trait} :
-    Notation.DoubleColon Self "from" := {
-    Notation.double_colon := from;
-  }.
-  
-  Global Instance I
-    : core.convert.From.Trait Self (T := ink.reflect.dispatch.DispatchError)
-      := {
-    core.convert.From.from `{H' : State.Trait} := from;
-  }.
-  Global Hint Resolve I : core.
-End Impl_core_convert_From_for_parity_scale_codec_error_Error.
 
 Module DecodeDispatch.
   Class Trait (Self : Set) `{parity_scale_codec.codec.Decode.Trait Self} :
@@ -3209,25 +2249,6 @@ Module Wrap_trait_def_1.
       End TraitDefinitionRegistry.
       Definition TraitDefinitionRegistry (E : Set) : Set :=
         TraitDefinitionRegistry.t (E := E).
-      
-      Module
-        Impl_ink_env_contract_ContractEnv_for_ink_reflect_trait_def_registry_TraitDefinitionRegistry_E.
-        Section
-          Impl_ink_env_contract_ContractEnv_for_ink_reflect_trait_def_registry_TraitDefinitionRegistry_E.
-          Context {E : Set}.
-          Definition Self :=
-            ink.reflect.trait_def.registry.TraitDefinitionRegistry E.
-          
-          Definition Env : Set := E.
-          
-          Global Instance I : ink_env.contract.ContractEnv.Trait Self := {
-            ink_env.contract.ContractEnv.Env := Env;
-          }.
-        End
-          Impl_ink_env_contract_ContractEnv_for_ink_reflect_trait_def_registry_TraitDefinitionRegistry_E.
-        Global Hint Resolve I : core.
-      End
-        Impl_ink_env_contract_ContractEnv_for_ink_reflect_trait_def_registry_TraitDefinitionRegistry_E.
     End registry.
   End trait_def.
 End Wrap_trait_def_1.
@@ -3332,25 +2353,6 @@ Module registry.
   End TraitDefinitionRegistry.
   Definition TraitDefinitionRegistry (E : Set) : Set :=
     TraitDefinitionRegistry.t (E := E).
-  
-  Module
-    Impl_ink_env_contract_ContractEnv_for_ink_reflect_trait_def_registry_TraitDefinitionRegistry_E.
-    Section
-      Impl_ink_env_contract_ContractEnv_for_ink_reflect_trait_def_registry_TraitDefinitionRegistry_E.
-      Context {E : Set}.
-      Definition Self :=
-        ink.reflect.trait_def.registry.TraitDefinitionRegistry E.
-      
-      Definition Env : Set := E.
-      
-      Global Instance I : ink_env.contract.ContractEnv.Trait Self := {
-        ink_env.contract.ContractEnv.Env := Env;
-      }.
-    End
-      Impl_ink_env_contract_ContractEnv_for_ink_reflect_trait_def_registry_TraitDefinitionRegistry_E.
-    Global Hint Resolve I : core.
-  End
-    Impl_ink_env_contract_ContractEnv_for_ink_reflect_trait_def_registry_TraitDefinitionRegistry_E.
 End registry.
 
 Module TraitDefinitionRegistry.
@@ -3372,24 +2374,6 @@ Module TraitDefinitionRegistry.
 End TraitDefinitionRegistry.
 Definition TraitDefinitionRegistry (E : Set) : Set :=
   TraitDefinitionRegistry.t (E := E).
-
-Module
-  Impl_ink_env_contract_ContractEnv_for_ink_reflect_trait_def_registry_TraitDefinitionRegistry_E.
-  Section
-    Impl_ink_env_contract_ContractEnv_for_ink_reflect_trait_def_registry_TraitDefinitionRegistry_E.
-    Context {E : Set}.
-    Definition Self := ink.reflect.trait_def.registry.TraitDefinitionRegistry E.
-    
-    Definition Env : Set := E.
-    
-    Global Instance I : ink_env.contract.ContractEnv.Trait Self := {
-      ink_env.contract.ContractEnv.Env := Env;
-    }.
-  End
-    Impl_ink_env_contract_ContractEnv_for_ink_reflect_trait_def_registry_TraitDefinitionRegistry_E.
-  Global Hint Resolve I : core.
-End
-  Impl_ink_env_contract_ContractEnv_for_ink_reflect_trait_def_registry_TraitDefinitionRegistry_E.
 
 Module chain_extension.
   Module ChainExtensionInstance.
@@ -3436,7 +2420,7 @@ Module chain_extension.
     End OutputSealed.
   End private.
   
-  Module IsResultType.
+  (* Module IsResultType.
     Class Trait
         (Self : Set)
         `{ink.chain_extension.private.IsResultSealed.Trait Self} :
@@ -3452,40 +2436,7 @@ Module chain_extension.
       : Notation.DoubleColonType Self "Err" := {
       Notation.double_colon_type := Err;
     }.
-  End IsResultType.
-  
-  Module
-    Impl_ink_chain_extension_private_IsResultSealed_for_core_result_Result_T_E.
-    Section
-      Impl_ink_chain_extension_private_IsResultSealed_for_core_result_Result_T_E.
-      Context {T E : Set}.
-      Definition Self := core.result.Result T E.
-      
-      Global Instance I
-        : ink.chain_extension.private.IsResultSealed.Trait Self := {
-      }.
-    End
-      Impl_ink_chain_extension_private_IsResultSealed_for_core_result_Result_T_E.
-    Global Hint Resolve I : core.
-  End
-    Impl_ink_chain_extension_private_IsResultSealed_for_core_result_Result_T_E.
-  
-  Module Impl_ink_chain_extension_IsResultType_for_core_result_Result_T_E.
-    Section Impl_ink_chain_extension_IsResultType_for_core_result_Result_T_E.
-      Context {T E : Set}.
-      Definition Self := core.result.Result T E.
-      
-      Definition Ok : Set := T.
-      
-      Definition Err : Set := E.
-      
-      Global Instance I : ink.chain_extension.IsResultType.Trait Self := {
-        ink.chain_extension.IsResultType.Ok := Ok;
-        ink.chain_extension.IsResultType.Err := Err;
-      }.
-    End Impl_ink_chain_extension_IsResultType_for_core_result_Result_T_E.
-    Global Hint Resolve I : core.
-  End Impl_ink_chain_extension_IsResultType_for_core_result_Result_T_E.
+  End IsResultType. *)
   
   Module Output.
     Class Trait
@@ -3506,48 +2457,6 @@ Module chain_extension.
     Inductive t : Set := Build.
   End ValueReturned.
   Definition ValueReturned := @ValueReturned.t.
-  
-  Module
-    Impl_ink_chain_extension_private_OutputSealed_for_ink_chain_extension_ValueReturned.
-    Definition Self := ink.chain_extension.ValueReturned.
-    
-    Global Instance I : ink.chain_extension.private.OutputSealed.Trait Self := {
-    }.
-    Global Hint Resolve I : core.
-  End
-    Impl_ink_chain_extension_private_OutputSealed_for_ink_chain_extension_ValueReturned.
-  
-  Module Impl_ink_chain_extension_Output_for_ink_chain_extension_ValueReturned.
-    Section
-      Impl_ink_chain_extension_Output_for_ink_chain_extension_ValueReturned.
-      Context {T E : Set}.
-      Definition Self := ink.chain_extension.ValueReturned.
-      
-      Definition ReturnType : Set := T.
-      
-      Global Instance I
-        : ink.chain_extension.Output.Trait Self (T := T) (E := E) := {
-        ink.chain_extension.Output.ReturnType := ReturnType;
-      }.
-    End Impl_ink_chain_extension_Output_for_ink_chain_extension_ValueReturned.
-    Global Hint Resolve I : core.
-  End Impl_ink_chain_extension_Output_for_ink_chain_extension_ValueReturned.
-  
-  Module Impl_ink_chain_extension_Output_for_ink_chain_extension_ValueReturned.
-    Section
-      Impl_ink_chain_extension_Output_for_ink_chain_extension_ValueReturned.
-      Context {T E : Set}.
-      Definition Self := ink.chain_extension.ValueReturned.
-      
-      Definition ReturnType : Set := core.result.Result T E.
-      
-      Global Instance I
-        : ink.chain_extension.Output.Trait Self (T := T) (E := E) := {
-        ink.chain_extension.Output.ReturnType := ReturnType;
-      }.
-    End Impl_ink_chain_extension_Output_for_ink_chain_extension_ValueReturned.
-    Global Hint Resolve I : core.
-  End Impl_ink_chain_extension_Output_for_ink_chain_extension_ValueReturned.
 End chain_extension.
 
 Module ChainExtensionInstance.
@@ -3578,7 +2487,7 @@ Module ChainExtension.
   }.
 End ChainExtension.
 
-Module IsResultType.
+(* Module IsResultType.
   Class Trait
       (Self : Set)
       `{ink.chain_extension.private.IsResultSealed.Trait Self} :
@@ -3593,39 +2502,7 @@ Module IsResultType.
   Global Instance Method_Err `(Trait) : Notation.DoubleColonType Self "Err" := {
     Notation.double_colon_type := Err;
   }.
-End IsResultType.
-
-Module
-  Impl_ink_chain_extension_private_IsResultSealed_for_core_result_Result_T_E.
-  Section
-    Impl_ink_chain_extension_private_IsResultSealed_for_core_result_Result_T_E.
-    Context {T E : Set}.
-    Definition Self := core.result.Result T E.
-    
-    Global Instance I
-      : ink.chain_extension.private.IsResultSealed.Trait Self := {
-    }.
-  End
-    Impl_ink_chain_extension_private_IsResultSealed_for_core_result_Result_T_E.
-  Global Hint Resolve I : core.
-End Impl_ink_chain_extension_private_IsResultSealed_for_core_result_Result_T_E.
-
-Module Impl_ink_chain_extension_IsResultType_for_core_result_Result_T_E.
-  Section Impl_ink_chain_extension_IsResultType_for_core_result_Result_T_E.
-    Context {T E : Set}.
-    Definition Self := core.result.Result T E.
-    
-    Definition Ok : Set := T.
-    
-    Definition Err : Set := E.
-    
-    Global Instance I : ink.chain_extension.IsResultType.Trait Self := {
-      ink.chain_extension.IsResultType.Ok := Ok;
-      ink.chain_extension.IsResultType.Err := Err;
-    }.
-  End Impl_ink_chain_extension_IsResultType_for_core_result_Result_T_E.
-  Global Hint Resolve I : core.
-End Impl_ink_chain_extension_IsResultType_for_core_result_Result_T_E.
+End IsResultType. *)
 
 Module Output.
   Class Trait
@@ -3646,46 +2523,6 @@ Module ValueReturned.
   Inductive t : Set := Build.
 End ValueReturned.
 Definition ValueReturned := @ValueReturned.t.
-
-Module
-  Impl_ink_chain_extension_private_OutputSealed_for_ink_chain_extension_ValueReturned.
-  Definition Self := ink.chain_extension.ValueReturned.
-  
-  Global Instance I : ink.chain_extension.private.OutputSealed.Trait Self := {
-  }.
-  Global Hint Resolve I : core.
-End
-  Impl_ink_chain_extension_private_OutputSealed_for_ink_chain_extension_ValueReturned.
-
-Module Impl_ink_chain_extension_Output_for_ink_chain_extension_ValueReturned.
-  Section Impl_ink_chain_extension_Output_for_ink_chain_extension_ValueReturned.
-    Context {T E : Set}.
-    Definition Self := ink.chain_extension.ValueReturned.
-    
-    Definition ReturnType : Set := T.
-    
-    Global Instance I
-      : ink.chain_extension.Output.Trait Self (T := T) (E := E) := {
-      ink.chain_extension.Output.ReturnType := ReturnType;
-    }.
-  End Impl_ink_chain_extension_Output_for_ink_chain_extension_ValueReturned.
-  Global Hint Resolve I : core.
-End Impl_ink_chain_extension_Output_for_ink_chain_extension_ValueReturned.
-
-Module Impl_ink_chain_extension_Output_for_ink_chain_extension_ValueReturned.
-  Section Impl_ink_chain_extension_Output_for_ink_chain_extension_ValueReturned.
-    Context {T E : Set}.
-    Definition Self := ink.chain_extension.ValueReturned.
-    
-    Definition ReturnType : Set := core.result.Result T E.
-    
-    Global Instance I
-      : ink.chain_extension.Output.Trait Self (T := T) (E := E) := {
-      ink.chain_extension.Output.ReturnType := ReturnType;
-    }.
-  End Impl_ink_chain_extension_Output_for_ink_chain_extension_ValueReturned.
-  Global Hint Resolve I : core.
-End Impl_ink_chain_extension_Output_for_ink_chain_extension_ValueReturned.
 
 Module Wrap_private_1.
   Module private.
@@ -3771,79 +2608,6 @@ Module env_access.
     End EnvAccess.
   End EnvAccess.
   Definition EnvAccess (E : Set) : Set := EnvAccess.t (E := E).
-  
-  Module Impl_core_marker_Copy_for_ink_env_access_EnvAccess_E.
-    Section Impl_core_marker_Copy_for_ink_env_access_EnvAccess_E.
-      Context {E : Set}.
-      Definition Self := ink.env_access.EnvAccess E.
-      
-      Global Instance I : core.marker.Copy.Trait Self := {
-      }.
-    End Impl_core_marker_Copy_for_ink_env_access_EnvAccess_E.
-    Global Hint Resolve I : core.
-  End Impl_core_marker_Copy_for_ink_env_access_EnvAccess_E.
-  
-  Module Impl_core_clone_Clone_for_ink_env_access_EnvAccess_E.
-    Section Impl_core_clone_Clone_for_ink_env_access_EnvAccess_E.
-      Context {E : Set}.
-      Definition Self := ink.env_access.EnvAccess E.
-      
-      Parameter clone :
-          forall `{H' : State.Trait},
-          (ref Self) -> M (H := H') (ink.env_access.EnvAccess E).
-      
-      Global Instance Method_clone `{H' : State.Trait} :
-        Notation.Dot "clone" := {
-        Notation.dot := clone;
-      }.
-      
-      Global Instance I : core.clone.Clone.Trait Self := {
-        core.clone.Clone.clone `{H' : State.Trait} := clone;
-      }.
-    End Impl_core_clone_Clone_for_ink_env_access_EnvAccess_E.
-    Global Hint Resolve I : core.
-  End Impl_core_clone_Clone_for_ink_env_access_EnvAccess_E.
-  
-  Module Impl_core_default_Default_for_ink_env_access_EnvAccess_E.
-    Section Impl_core_default_Default_for_ink_env_access_EnvAccess_E.
-      Context {E : Set}.
-      Definition Self := ink.env_access.EnvAccess E.
-      
-      Parameter default : forall `{H' : State.Trait}, M (H := H') Self.
-      
-      Global Instance AssociatedFunction_default `{H' : State.Trait} :
-        Notation.DoubleColon Self "default" := {
-        Notation.double_colon := default;
-      }.
-      
-      Global Instance I : core.default.Default.Trait Self := {
-        core.default.Default.default `{H' : State.Trait} := default;
-      }.
-    End Impl_core_default_Default_for_ink_env_access_EnvAccess_E.
-    Global Hint Resolve I : core.
-  End Impl_core_default_Default_for_ink_env_access_EnvAccess_E.
-  
-  Module Impl_core_fmt_Debug_for_ink_env_access_EnvAccess_E.
-    Section Impl_core_fmt_Debug_for_ink_env_access_EnvAccess_E.
-      Context {E : Set}.
-      Definition Self := ink.env_access.EnvAccess E.
-      
-      Parameter fmt :
-          forall `{H' : State.Trait},
-          (ref Self) ->
-            (mut_ref core.fmt.Formatter) ->
-            M (H := H') core.fmt.Result.
-      
-      Global Instance Method_fmt `{H' : State.Trait} : Notation.Dot "fmt" := {
-        Notation.dot := fmt;
-      }.
-      
-      Global Instance I : core.fmt.Debug.Trait Self := {
-        core.fmt.Debug.fmt `{H' : State.Trait} := fmt;
-      }.
-    End Impl_core_fmt_Debug_for_ink_env_access_EnvAccess_E.
-    Global Hint Resolve I : core.
-  End Impl_core_fmt_Debug_for_ink_env_access_EnvAccess_E.
 End env_access.
 
 Module EnvAccess.
@@ -3864,75 +2628,3 @@ Module EnvAccess.
   End EnvAccess.
 End EnvAccess.
 Definition EnvAccess (E : Set) : Set := EnvAccess.t (E := E).
-
-Module Impl_core_marker_Copy_for_ink_env_access_EnvAccess_E.
-  Section Impl_core_marker_Copy_for_ink_env_access_EnvAccess_E.
-    Context {E : Set}.
-    Definition Self := ink.env_access.EnvAccess E.
-    
-    Global Instance I : core.marker.Copy.Trait Self := {
-    }.
-  End Impl_core_marker_Copy_for_ink_env_access_EnvAccess_E.
-  Global Hint Resolve I : core.
-End Impl_core_marker_Copy_for_ink_env_access_EnvAccess_E.
-
-Module Impl_core_clone_Clone_for_ink_env_access_EnvAccess_E.
-  Section Impl_core_clone_Clone_for_ink_env_access_EnvAccess_E.
-    Context {E : Set}.
-    Definition Self := ink.env_access.EnvAccess E.
-    
-    Parameter clone :
-        forall `{H' : State.Trait},
-        (ref Self) -> M (H := H') (ink.env_access.EnvAccess E).
-    
-    Global Instance Method_clone `{H' : State.Trait} : Notation.Dot "clone" := {
-      Notation.dot := clone;
-    }.
-    
-    Global Instance I : core.clone.Clone.Trait Self := {
-      core.clone.Clone.clone `{H' : State.Trait} := clone;
-    }.
-  End Impl_core_clone_Clone_for_ink_env_access_EnvAccess_E.
-  Global Hint Resolve I : core.
-End Impl_core_clone_Clone_for_ink_env_access_EnvAccess_E.
-
-Module Impl_core_default_Default_for_ink_env_access_EnvAccess_E.
-  Section Impl_core_default_Default_for_ink_env_access_EnvAccess_E.
-    Context {E : Set}.
-    Definition Self := ink.env_access.EnvAccess E.
-    
-    Parameter default : forall `{H' : State.Trait}, M (H := H') Self.
-    
-    Global Instance AssociatedFunction_default `{H' : State.Trait} :
-      Notation.DoubleColon Self "default" := {
-      Notation.double_colon := default;
-    }.
-    
-    Global Instance I : core.default.Default.Trait Self := {
-      core.default.Default.default `{H' : State.Trait} := default;
-    }.
-  End Impl_core_default_Default_for_ink_env_access_EnvAccess_E.
-  Global Hint Resolve I : core.
-End Impl_core_default_Default_for_ink_env_access_EnvAccess_E.
-
-Module Impl_core_fmt_Debug_for_ink_env_access_EnvAccess_E.
-  Section Impl_core_fmt_Debug_for_ink_env_access_EnvAccess_E.
-    Context {E : Set}.
-    Definition Self := ink.env_access.EnvAccess E.
-    
-    Parameter fmt :
-        forall `{H' : State.Trait},
-        (ref Self) ->
-          (mut_ref core.fmt.Formatter) ->
-          M (H := H') core.fmt.Result.
-    
-    Global Instance Method_fmt `{H' : State.Trait} : Notation.Dot "fmt" := {
-      Notation.dot := fmt;
-    }.
-    
-    Global Instance I : core.fmt.Debug.Trait Self := {
-      core.fmt.Debug.fmt `{H' : State.Trait} := fmt;
-    }.
-  End Impl_core_fmt_Debug_for_ink_env_access_EnvAccess_E.
-  Global Hint Resolve I : core.
-End Impl_core_fmt_Debug_for_ink_env_access_EnvAccess_E.
